thys/Datatype_TVsubst.thy
@@ -281,7 +281,7 @@ for
   subgoal by (rule emp_bound)
   subgoal
     using emp_bound IImsupp_SSupp_bound Rep_SSfun by auto 
-  subgoal unfolding swapping_def apply safe
+  subgoal unfolding termLikeStr_def apply safe
     subgoal by simp
     subgoal premises prems for u v
       supply prems[transfer_rule] bij_comp[transfer_rule] supp_comp_bound[transfer_rule]
@@ -347,7 +347,7 @@ for
       done
     done
   subgoal
-    unfolding swappingC_def apply (intro conjI)
+    unfolding termLikeStrC_def apply (intro conjI)
     subgoal by (auto simp: map_TT_id)
     subgoal by (safe, transfer') (auto simp: asSS_def T_map_comp supp_comp_bound)
     subgoal by (safe, transfer') (auto simp: asSS_def supp_id_bound intro!: alpha_bij[of _ _ _ id, unfolded T_map_id] alpha_refl)
